src/Compare.v
@@ -1,0 +1,55 @@
+Require Import Prog.
+Require Import BasicProg.
+Require Import SepAuto.
+Require Import Word.
+Require Import Hoare.
+Require Import Pred.
+Require Import EqdepFacts.
+
+Set Implicit Arguments.
+
+Definition compare T sz (buf1 buf2 : word sz) rx : prog T :=
+  If (weq buf1 buf2) {
+    rx true
+  } else {
+    rx false
+  }.
+
+
+Theorem compare_ok :
+  forall sz (buf1 buf2 : word sz),
+  {< (_ : unit),
+  PRE         emp
+  POST RET:r  emp * [[ r = true -> buf1 = buf2 ]] * [[ r = false -> buf1 <> buf2 ]]
+  CRASH       emp
+  >} compare buf1 buf2.
+Proof.
+  unfold compare. step. step. step.
+Qed.
+
+Definition compare_hash T sz (buf1 buf2 : word sz) rx : prog T :=
+  h1 <- Hash buf1;
+  h2 <- Hash buf2;
+  If (weq h1 h2) {
+    rx true
+  } else {
+    rx false
+  }.
+
+Theorem compare_hash_ok :
+  forall sz (buf1 buf2 : word sz),
+  {< (_ : unit),
+  PRE         emp
+  POST RET:r  emp * [[ r = true -> buf1 = buf2 ]] * [[ r = false -> buf1 <> buf2 ]]
+  CRASH       emp
+  >} compare_hash buf1 buf2.
+Proof.
+  unfold compare_hash. step. step. step.
+  step. rewrite H5 in H7. rewrite H7 in H8.
+  pose proof (eq_sigT_snd H8).
+  autorewrite with core in *. auto.
+  step.
+
+  Grab Existential Variables.
+  all: eauto.
+Qed.
